WIP: sim upto

src/FairSim.v
@@ -6,6 +6,7 @@ Export ITreeNotations.
 
 Require Import Coq.Classes.RelationClasses.
 Require Import Program.
+Require Import Lia.
 
 From Fairness Require Import ITreeLib.
 From Fairness Require Import FairBeh.
@@ -19,8 +20,7 @@ Section SIM.
   (* Definition stuck_idx (m: imap) (j: id) := le (m j) 0. *)
 
   Inductive _sim
-            (sim: forall R0 R1 (RR: R0 -> R1 -> Prop),
-                bool -> imap -> bool  -> imap -> (@state _ R0) -> (@state _ R1) -> Prop)
+            (sim: forall R0 R1 (RR: R0 -> R1 -> Prop), bool -> imap -> bool  -> imap -> (@state _ R0) -> (@state _ R1) -> Prop)
             {R0 R1} (RR: R0 -> R1 -> Prop) (p_src: bool) (m_src: imap) (p_tgt: bool) (m_tgt: imap) :
     (@state _ R0) -> (@state _ R1) -> Prop :=
   | sim_ret
@@ -29,36 +29,30 @@ Section SIM.
     :
     _sim sim RR p_src m_src p_tgt m_tgt (Ret r_src) (Ret r_tgt)
   | sim_obs
-      m_src0 m_tgt0 ktr_src0 ktr_tgt0 fn args
+      ktr_src0 ktr_tgt0 fn args
       (SIM: forall r_src r_tgt (EQ: r_src = r_tgt),
-          sim _ _ RR true m_src0 true m_tgt0 (ktr_src0 r_src) (ktr_tgt0 r_tgt))
-      (ISRC: soft_update m_src m_src0)
-      (ITGT: soft_update m_tgt m_tgt0)
+          sim _ _ RR true m_src true m_tgt (ktr_src0 r_src) (ktr_tgt0 r_tgt))
     :
     _sim sim RR p_src m_src p_tgt m_tgt (Vis (Observe fn args) ktr_src0) (Vis (Observe fn args) ktr_tgt0)
 
   | sim_tauL
-      m_src0 itr_src0 itr_tgt0
-      (SIM: @_sim sim _ _ RR true m_src0 p_tgt m_tgt itr_src0 itr_tgt0)
-      (ISRC: soft_update m_src m_src0)
+      itr_src0 itr_tgt0
+      (SIM: @_sim sim _ _ RR true m_src p_tgt m_tgt itr_src0 itr_tgt0)
     :
     _sim sim RR p_src m_src p_tgt m_tgt (Tau itr_src0) itr_tgt0
   | sim_tauR
-      m_tgt0 itr_src0 itr_tgt0
-      (SIM: @_sim sim _ _ RR p_src m_src true m_tgt0 itr_src0 itr_tgt0)
-      (ITGT: soft_update m_tgt m_tgt0)
+      itr_src0 itr_tgt0
+      (SIM: @_sim sim _ _ RR p_src m_src true m_tgt itr_src0 itr_tgt0)
     :
     _sim sim RR p_src m_src p_tgt m_tgt itr_src0 (Tau itr_tgt0)
   | sim_chooseL
-      m_src0 X ktr_src0 itr_tgt0
-      (SIM: exists x, _sim sim RR true m_src0 p_tgt m_tgt (ktr_src0 x) itr_tgt0)
-      (ISRC: soft_update m_src m_src0)
+      X ktr_src0 itr_tgt0
+      (SIM: exists x, _sim sim RR true m_src p_tgt m_tgt (ktr_src0 x) itr_tgt0)
     :
     _sim sim RR p_src m_src p_tgt m_tgt (trigger (Choose X) >>= ktr_src0) itr_tgt0
   | sim_chooseR
-      m_tgt0 X itr_src0 ktr_tgt0
-      (SIM: forall x, _sim sim RR p_src m_src true m_tgt0 itr_src0 (ktr_tgt0 x))
-      (ITGT: soft_update m_tgt m_tgt0)
+      X itr_src0 ktr_tgt0
+      (SIM: forall x, _sim sim RR p_src m_src true m_tgt itr_src0 (ktr_tgt0 x))
     :
     _sim sim RR p_src m_src p_tgt m_tgt itr_src0 (trigger (Choose X) >>= ktr_tgt0)
 
@@ -80,7 +74,6 @@ Section SIM.
       (SIM: sim _ _ RR false m_src0 false m_tgt0 itr_src0 itr_tgt0)
       (PSRC: p_src = true)
       (PTGT: p_tgt = true)
-      (* (IMAP: forall i, (<<SSRC: stuck_idx m_src i>>) -> (<<STGT: stuck_idx m_tgt i>>)) *)
     :
     _sim sim RR p_src m_src p_tgt m_tgt itr_src0 itr_tgt0
 
@@ -90,7 +83,7 @@ Section SIM.
     _sim sim RR p_src m_src p_tgt m_tgt (trigger Undefined >>= ktr_src0) itr_tgt0
   .
 
-  Lemma _sim_ind2 (r: forall R0 R1 (RR: R0 -> R1 -> Prop), bool -> imap  -> bool -> imap -> (@state _ R0) -> (@state _ R1) -> Prop)
+  Lemma sim_ind (r: forall R0 R1 (RR: R0 -> R1 -> Prop), bool -> imap  -> bool -> imap -> (@state _ R0) -> (@state _ R1) -> Prop)
         R0 R1 (RR: R0 -> R1 -> Prop)
         (P: bool -> imap  -> bool -> imap -> (@state _ R0) -> (@state _ R1) -> Prop)
         (RET: forall
@@ -99,37 +92,31 @@ Section SIM.
             (SIM: RR r_src r_tgt),
             P p_src m_src p_tgt m_tgt (Ret r_src) (Ret r_tgt))
         (OBS: forall
-            p_src m_src p_tgt m_tgt m_src0 m_tgt0 ktr_src0 ktr_tgt0
+            p_src m_src p_tgt m_tgt ktr_src0 ktr_tgt0
             fn args
-            (SIM: forall r_src r_tgt (EQ: r_src = r_tgt), r _ _ RR true m_src0 true m_tgt0 (ktr_src0 r_src) (ktr_tgt0 r_tgt))
-            (ISRC: soft_update m_src m_src0)
-            (ITGT: soft_update m_tgt m_tgt0),
+            (SIM: forall r_src r_tgt (EQ: r_src = r_tgt), r _ _ RR true m_src true m_tgt (ktr_src0 r_src) (ktr_tgt0 r_tgt)),
             P p_src m_src p_tgt m_tgt (Vis (Observe fn args) ktr_src0) (Vis (Observe fn args) ktr_tgt0))
         (TAUL: forall 
-            p_src m_src p_tgt m_tgt m_src0 itr_src0 itr_tgt0
-            (SIM: _sim r RR true m_src0 p_tgt m_tgt itr_src0 itr_tgt0)
-            (IH: P true m_src0 p_tgt m_tgt itr_src0 itr_tgt0)
-            (ISRC: soft_update m_src m_src0),
+            p_src m_src p_tgt m_tgt itr_src0 itr_tgt0
+            (SIM: _sim r RR true m_src p_tgt m_tgt itr_src0 itr_tgt0)
+            (IH: P true m_src p_tgt m_tgt itr_src0 itr_tgt0),
             P p_src m_src p_tgt m_tgt (Tau itr_src0) itr_tgt0)
         (TAUR: forall 
-            p_src m_src p_tgt m_tgt m_tgt0 itr_src0 itr_tgt0
-            (SIM: _sim r RR p_src m_src true m_tgt0 itr_src0 itr_tgt0)
-            (IH: P p_src m_src true m_tgt0 itr_src0 itr_tgt0)
-            (ITGT: soft_update m_tgt m_tgt0),
+            p_src m_src p_tgt m_tgt itr_src0 itr_tgt0
+            (SIM: _sim r RR p_src m_src true m_tgt itr_src0 itr_tgt0)
+            (IH: P p_src m_src true m_tgt itr_src0 itr_tgt0),
             P p_src m_src p_tgt m_tgt itr_src0 (Tau itr_tgt0))
         (CHOOSEL: forall
-            p_src m_src p_tgt m_tgt m_src0 X ktr_src0 itr_tgt0
+            p_src m_src p_tgt m_tgt X ktr_src0 itr_tgt0
             (SIM: exists x,
-                (<<SIM: _sim r RR true m_src0 p_tgt m_tgt (ktr_src0 x) itr_tgt0>>) /\
-                  (<<IH: P true m_src0 p_tgt m_tgt (ktr_src0 x) itr_tgt0>>))
-            (ISRC: soft_update m_src m_src0),
+                (<<SIM: _sim r RR true m_src p_tgt m_tgt (ktr_src0 x) itr_tgt0>>) /\
+                  (<<IH: P true m_src p_tgt m_tgt (ktr_src0 x) itr_tgt0>>)),
             P p_src m_src p_tgt m_tgt (ITree.bind (trigger (Choose X)) ktr_src0) itr_tgt0)
         (CHOOSER: forall
-            p_src m_src p_tgt m_tgt m_tgt0 X itr_src0 ktr_tgt0
+            p_src m_src p_tgt m_tgt X itr_src0 ktr_tgt0
             (SIM: forall x,
-                (<<SIM: _sim r RR p_src m_src true m_tgt0 itr_src0 (ktr_tgt0 x)>>) /\
-                  (<<IH: P p_src m_src true m_tgt0 itr_src0 (ktr_tgt0 x)>>))
-            (ITGT: soft_update m_tgt m_tgt0),
+                (<<SIM: _sim r RR p_src m_src true m_tgt itr_src0 (ktr_tgt0 x)>>) /\
+                  (<<IH: P p_src m_src true m_tgt itr_src0 (ktr_tgt0 x)>>)),
             P p_src m_src p_tgt m_tgt itr_src0 (ITree.bind (trigger (Choose X)) ktr_tgt0))
         (FAIRL: forall
             p_src m_src p_tgt m_tgt f_src ktr_src0 itr_tgt0
@@ -149,7 +136,6 @@ Section SIM.
             (SIM: r _ _ RR false m_src0 false m_tgt0 itr_src0 itr_tgt0)
             (PSRC: p_src = true)
             (PTGT: p_tgt = true),
-            (* (IMAP: forall i, (<<SSRC: stuck_idx m_src i>>) -> (<<STGT: stuck_idx m_tgt i>>)) *)
             P p_src m_src p_tgt m_tgt itr_src0 itr_tgt0)
         (UB: forall
             p_src m_src p_tgt m_tgt ktr_src0 itr_tgt0,
@@ -176,7 +162,7 @@ Section SIM.
 
   Lemma sim_mon: monotone9 _sim.
   Proof.
-    ii. induction IN using _sim_ind2.
+    ii. induction IN using sim_ind.
     { econs 1; eauto. }
     { econs 2; eauto. }
     { econs 3; eauto. }
@@ -189,10 +175,258 @@ Section SIM.
     { econs 10; eauto. }
   Qed.
 
+  Hint Constructors _sim.
+  Hint Unfold sim.
   Hint Resolve sim_mon: paco.
   Hint Resolve cpn9_wcompat: paco.
 
+  Lemma sim_ind2 R0 R1 (RR: R0 -> R1 -> Prop)
+        (P: bool -> imap  -> bool -> imap -> (@state _ R0) -> (@state _ R1) -> Prop)
+        (RET: forall
+            p_src m_src p_tgt m_tgt
+            r_src r_tgt
+            (SIM: RR r_src r_tgt),
+            P p_src m_src p_tgt m_tgt (Ret r_src) (Ret r_tgt))
+        (OBS: forall
+            p_src m_src p_tgt m_tgt ktr_src0 ktr_tgt0
+            fn args
+            (SIM: forall r_src r_tgt (EQ: r_src = r_tgt), sim RR true m_src true m_tgt (ktr_src0 r_src) (ktr_tgt0 r_tgt)),
+            P p_src m_src p_tgt m_tgt (Vis (Observe fn args) ktr_src0) (Vis (Observe fn args) ktr_tgt0))
+        (TAUL: forall 
+            p_src m_src p_tgt m_tgt itr_src0 itr_tgt0
+            (SIM: sim RR true m_src p_tgt m_tgt itr_src0 itr_tgt0)
+            (IH: P true m_src p_tgt m_tgt itr_src0 itr_tgt0),
+            P p_src m_src p_tgt m_tgt (Tau itr_src0) itr_tgt0)
+        (TAUR: forall 
+            p_src m_src p_tgt m_tgt itr_src0 itr_tgt0
+            (SIM: sim RR p_src m_src true m_tgt itr_src0 itr_tgt0)
+            (IH: P p_src m_src true m_tgt itr_src0 itr_tgt0),
+            P p_src m_src p_tgt m_tgt itr_src0 (Tau itr_tgt0))
+        (CHOOSEL: forall
+            p_src m_src p_tgt m_tgt X ktr_src0 itr_tgt0
+            (SIM: exists x,
+                (<<SIM: sim RR true m_src p_tgt m_tgt (ktr_src0 x) itr_tgt0>>) /\
+                  (<<IH: P true m_src p_tgt m_tgt (ktr_src0 x) itr_tgt0>>)),
+            P p_src m_src p_tgt m_tgt (ITree.bind (trigger (Choose X)) ktr_src0) itr_tgt0)
+        (CHOOSER: forall
+            p_src m_src p_tgt m_tgt X itr_src0 ktr_tgt0
+            (SIM: forall x,
+                (<<SIM: sim RR p_src m_src true m_tgt itr_src0 (ktr_tgt0 x)>>) /\
+                  (<<IH: P p_src m_src true m_tgt itr_src0 (ktr_tgt0 x)>>)),
+            P p_src m_src p_tgt m_tgt itr_src0 (ITree.bind (trigger (Choose X)) ktr_tgt0))
+        (FAIRL: forall
+            p_src m_src p_tgt m_tgt f_src ktr_src0 itr_tgt0
+            (SIM: exists m_src0,
+                (<<FAIR: fair_update m_src m_src0 f_src>>) /\
+                  (<<SIM: sim RR true m_src0 p_tgt m_tgt (ktr_src0 tt) itr_tgt0>>) /\
+                  (<<IH: P true m_src0 p_tgt m_tgt (ktr_src0 tt) itr_tgt0>>)),
+            P p_src m_src p_tgt m_tgt (ITree.bind (trigger (Fair f_src)) ktr_src0) itr_tgt0)
+        (FAIRR: forall
+            p_src m_src p_tgt m_tgt f_tgt itr_src0 ktr_tgt0
+            (SIM: forall m_tgt0 (FAIR: fair_update m_tgt m_tgt0 f_tgt),
+                (<<SIM: sim RR p_src m_src true m_tgt0 itr_src0 (ktr_tgt0 tt)>>) /\
+                  (<<IH: P p_src m_src true m_tgt0 itr_src0 (ktr_tgt0 tt)>>)),
+            P p_src m_src p_tgt m_tgt itr_src0 (ITree.bind (trigger (Fair f_tgt)) ktr_tgt0))
+        (PROGRESS: forall
+            p_src m_src p_tgt m_tgt m_src0 m_tgt0 itr_src0 itr_tgt0
+            (SIM: sim RR false m_src0 false m_tgt0 itr_src0 itr_tgt0)
+            (PSRC: p_src = true)
+            (PTGT: p_tgt = true),
+            P p_src m_src p_tgt m_tgt itr_src0 itr_tgt0)
+        (UB: forall
+            p_src m_src p_tgt m_tgt ktr_src0 itr_tgt0,
+            P p_src m_src p_tgt m_tgt (ITree.bind (trigger Undefined) ktr_src0) itr_tgt0)
+    :
+    forall p_src m_src p_tgt m_tgt itr_src itr_tgt
+      (SIM: sim RR p_src m_src p_tgt m_tgt itr_src itr_tgt),
+      P p_src m_src p_tgt m_tgt itr_src itr_tgt.
+  Proof.
+    i. eapply sim_ind; i; eauto.
+    { eapply TAUL; eauto. pfold. eapply sim_mon; eauto. }
+    { eapply TAUR; eauto. pfold. eapply sim_mon; eauto. }
+    { eapply CHOOSEL; eauto. des. esplits; eauto. pfold. eapply sim_mon; eauto. }
+    { eapply CHOOSER; eauto. i. specialize (SIM0 x). des. esplits; eauto. pfold. eapply sim_mon; eauto. }
+    { eapply FAIRL; eauto. des. esplits; eauto. pfold. eapply sim_mon; eauto. }
+    { eapply FAIRR; eauto. i. eapply SIM0 in FAIR. des. esplits; eauto. pfold. eapply sim_mon; eauto. }
+    { clear - SIM. punfold SIM. eapply sim_mon; eauto. i. pclearbot. eauto. }
+  Qed.
+
+  (****************************************************)
+  (*********************** upto ***********************)
+  (****************************************************)
+
+  Variant sim_imap_ctxL
+          (sim: forall R0 R1: Type, (R0 -> R1 -> Prop) -> bool -> imap -> bool -> imap -> state -> state -> Prop)
+          R0 R1 (RR: R0 -> R1 -> Prop)
+    :
+    bool -> imap -> bool -> imap -> (@state _ R0) -> (@state _ R1) -> Prop :=
+    | sim_imap_ctxL_intro
+        msrc0 msrc1 mtgt psrc ptgt st_src st_tgt
+        (SIM: @sim _ _ RR psrc msrc1 ptgt mtgt st_src st_tgt)
+        (IMAP: soft_update msrc0 msrc1)
+      :
+      sim_imap_ctxL sim RR psrc msrc0 ptgt mtgt st_src st_tgt.
+
+  Lemma sim_imap_ctxL_mon: monotone9 sim_imap_ctxL.
+  Proof. ii. inv IN. econs; eauto. Qed.
+
+  Hint Resolve sim_imap_ctxL_mon: paco.
+
+  Lemma sim_imap_ctxL_wrepectful: wrespectful9 _sim sim_imap_ctxL.
+  Proof.
+    econs; eauto with paco.
+    i. inv PR. apply GF in SIM. depgen x4. induction SIM using sim_ind; i; eauto.
+    { econs. i. subst. eapply rclo9_clo_base. econs; eauto. }
+    { des. econs. eexists. eapply IH. eauto. }
+    { econs. i. specialize (SIM x). des. eapply IH. eauto. }
+    { econs. des. esplits.
+      2:{ eapply IH. reflexivity. }
+      clear - FAIR IMAP. unfold fair_update, soft_update in *. i. specialize (FAIR i). specialize (IMAP i). des_ifs; lia.
+    }
+    { econs. i. specialize (SIM m_tgt0). eapply SIM in FAIR. des. eauto. }
+    { clarify. eapply sim_mon; eauto. i. eapply rclo9_base. auto. }
+  Qed.
+
+  Lemma sim_imap_ctxL_spec: sim_imap_ctxL <10= gupaco9 _sim (cpn9 _sim).
+  Proof. i. eapply wrespect9_uclo; eauto with paco. eapply sim_imap_ctxL_wrepectful. Qed.
+
+
+
+  Variant sim_imap_ctxR
+          (sim: forall R0 R1: Type, (R0 -> R1 -> Prop) -> bool -> imap -> bool -> imap -> state -> state -> Prop)
+          R0 R1 (RR: R0 -> R1 -> Prop)
+    :
+    bool -> imap -> bool -> imap -> (@state _ R0) -> (@state _ R1) -> Prop :=
+    | sim_imap_ctxR_intro
+        msrc mtgt0 mtgt1 psrc ptgt st_src st_tgt
+        (SIM: @sim _ _ RR psrc msrc ptgt mtgt1 st_src st_tgt)
+        (IMAP: soft_update mtgt1 mtgt0)
+      :
+      sim_imap_ctxR sim RR psrc msrc ptgt mtgt0 st_src st_tgt.
+
+  Lemma sim_imap_ctxR_mon: monotone9 sim_imap_ctxR.
+  Proof. ii. inv IN. econs; eauto. Qed.
+
+  Hint Resolve sim_imap_ctxR_mon: paco.
+
+  Lemma sim_imap_ctxR_wrepectful: wrespectful9 _sim sim_imap_ctxR.
+  Proof.
+    econs; eauto with paco.
+    i. inv PR. apply GF in SIM. depgen x6. induction SIM using sim_ind; i; eauto.
+    { econs. i. subst. eapply rclo9_clo_base. econs; eauto. }
+    { des. econs. eexists. eauto. }
+    { econs. i. specialize (SIM x). des. eauto. }
+    { econs. des. esplits; eauto. }
+    { econs. i. hexploit SIM.
+      2:{ i; des. eapply IH. reflexivity. }
+      clear - IMAP FAIR. unfold fair_update, soft_update in *. i. specialize (IMAP i). specialize (FAIR i). des_ifs; lia.
+    }
+    { clarify. eapply sim_mon; eauto. i. eapply rclo9_base. auto. }
+  Qed.
+
+  Lemma sim_imap_ctxR_spec: sim_imap_ctxR <10= gupaco9 _sim (cpn9 _sim).
+  Proof. i. eapply wrespect9_uclo; eauto with paco. eapply sim_imap_ctxR_wrepectful. Qed.
+
+
+
+  Variant sim_indC
+          (sim: forall R0 R1: Type, (R0 -> R1 -> Prop) -> bool -> imap -> bool -> imap -> (@state _ R0) -> (@state _ R1) -> Prop)
+          R0 R1 (RR: R0 -> R1 -> Prop) (p_src: bool) (m_src: imap) (p_tgt: bool) (m_tgt: imap)
+    :
+    (@state _ R0) -> (@state _ R1) -> Prop :=
+    | sim_indC_ret
+        r_src r_tgt
+        (SIM: RR r_src r_tgt)
+      :
+      sim_indC sim RR p_src m_src p_tgt m_tgt (Ret r_src) (Ret r_tgt)
+    | sim_indC_obs
+        ktr_src0 ktr_tgt0 fn args
+        (SIM: forall r_src r_tgt (EQ: r_src = r_tgt),
+            sim _ _ RR true m_src true m_tgt (ktr_src0 r_src) (ktr_tgt0 r_tgt))
+      :
+      sim_indC sim RR p_src m_src p_tgt m_tgt (Vis (Observe fn args) ktr_src0) (Vis (Observe fn args) ktr_tgt0)
+
+    | sim_indC_tauL
+        itr_src0 itr_tgt0
+        (SIM: sim _ _ RR true m_src p_tgt m_tgt itr_src0 itr_tgt0)
+      :
+      sim_indC sim RR p_src m_src p_tgt m_tgt (Tau itr_src0) itr_tgt0
+    | sim_indC_tauR
+        itr_src0 itr_tgt0
+        (SIM: sim _ _ RR p_src m_src true m_tgt itr_src0 itr_tgt0)
+      :
+      sim_indC sim RR p_src m_src p_tgt m_tgt itr_src0 (Tau itr_tgt0)
+    | sim_indC_chooseL
+        X ktr_src0 itr_tgt0
+        (SIM: exists x, sim _ _ RR true m_src p_tgt m_tgt (ktr_src0 x) itr_tgt0)
+      :
+      sim_indC sim RR p_src m_src p_tgt m_tgt (trigger (Choose X) >>= ktr_src0) itr_tgt0
+    | sim_indC_chooseR
+        X itr_src0 ktr_tgt0
+        (SIM: forall x, sim _ _ RR p_src m_src true m_tgt itr_src0 (ktr_tgt0 x))
+      :
+      sim_indC sim RR p_src m_src p_tgt m_tgt itr_src0 (trigger (Choose X) >>= ktr_tgt0)
+
+    | sim_indC_fairL
+        f_src ktr_src0 itr_tgt0
+        (SIM: exists m_src0, (<<FAIR: fair_update m_src m_src0 f_src>>) /\
+                          (<<SIM: sim _ _ RR true m_src0 p_tgt m_tgt (ktr_src0 tt) itr_tgt0>>))
+      :
+      sim_indC sim RR p_src m_src p_tgt m_tgt (trigger (Fair f_src) >>= ktr_src0) itr_tgt0
+    | sim_indC_fairR
+        f_tgt itr_src0 ktr_tgt0
+        (SIM: forall m_tgt0 (FAIR: fair_update m_tgt m_tgt0 f_tgt),
+            sim _ _ RR p_src m_src true m_tgt0 itr_src0 (ktr_tgt0 tt))
+      :
+      sim_indC sim RR p_src m_src p_tgt m_tgt itr_src0 (trigger (Fair f_tgt) >>= ktr_tgt0)
+
+    | sim_indC_progress
+        itr_src0 itr_tgt0 m_src0 m_tgt0
+        (SIM: sim _ _ RR false m_src0 false m_tgt0 itr_src0 itr_tgt0)
+        (PSRC: p_src = true)
+        (PTGT: p_tgt = true)
+      :
+      sim_indC sim RR p_src m_src p_tgt m_tgt itr_src0 itr_tgt0
+
+    | sim_indC_ub
+        ktr_src0 itr_tgt0
+      :
+      sim_indC sim RR p_src m_src p_tgt m_tgt (trigger Undefined >>= ktr_src0) itr_tgt0
+  .
+
+  Lemma sim_indC_mon: monotone9 sim_indC.
+  Proof.
+    ii. inv IN.
+    1,2,3,4,5,6,7,8,9: econs; eauto.
+    { des; eauto. }
+    { des; esplits; eauto. }
+    { econs 10. }
+  Qed.
+
+  Hint Resolve sim_indC_mon: paco.
+
+  Lemma sim_indC_wrepectful: wrespectful9 _sim sim_indC.
+  Proof.
+    econs; eauto with paco.
+    i. inv PR; eauto.
+    { econs; eauto. i. eapply rclo9_base. eauto. }
+    { econs; eauto. eapply sim_mon; eauto. i. eapply rclo9_base. auto. }
+    { econs; eauto. eapply sim_mon; eauto. i. eapply rclo9_base. auto. }
+    { econs; eauto. des. eexists. eapply sim_mon; eauto. i. eapply rclo9_base. auto. }
+    { econs; eauto. i. eapply sim_mon; eauto. i. eapply rclo9_base. auto. }
+    { econs; eauto. des. esplits; eauto. eapply sim_mon; eauto. i. eapply rclo9_base. auto. }
+    { econs; eauto. i. eapply sim_mon; eauto. i. eapply rclo9_base. auto. }
+    { eapply sim_mon. econs 9; eauto. i. eapply rclo9_base. auto. }
+  Qed.
+
+  Lemma sim_indC_spec: sim_indC <10= gupaco9 _sim (cpn9 _sim).
+  Proof. i. eapply wrespect9_uclo; eauto with paco. eapply sim_indC_wrepectful. Qed.
+
 End SIM.
+#[export] Hint Constructors _sim.
+#[export] Hint Unfold sim.
+#[export] Hint Resolve sim_mon: paco.
+#[export] Hint Resolve cpn9_wcompat: paco.
 
 
 
@@ -248,6 +482,36 @@ Section EX.
   Goal sim RR false imsrc1 false imtgt1 src1 tgt1.
   Proof.
     unfold src1, tgt1.
+    ginit. gcofix CIH. rewrite unfold_while_itree. ired.
+    guclo sim_indC_spec. econs 8. i.
+    guclo sim_indC_spec. econs.
+    guclo sim_imap_ctxR_spec. econs.
+    { rewrite unfold_while_itree. ired. guclo sim_indC_spec. econs. i.
+      instantiate (1:=fun id => 0) in FAIR0.
+      exfalso. unfold fair_update in FAIR0. specialize FAIR0 with 0. ss. lia.
+    }
+    
+    
+
+
+      inv FAIR0.
+      exfalso. unfold update_
+
+    
+    guclo sim_indC_spec. econs 8. i.
+    guclo sim_imap_ctxR_spec. econs.
+    { guclo sim_indC_spec. econs. 
+
+      instantiate (1:= fun id => 0).
+
+    gstep. rewrite unfold_while_itree. ired.
+    econs 8. i. guclo sim_imap_ctxR.
+
+    econs.
+    
+
+
+    
     pcofix CIH. pfold. rewrite unfold_while_itree. ired.
     econs 8. i.
     econs.
